Fixed issues with decidability of the signature

theories/Extraction/Subtyping.v
@@ -21,16 +21,17 @@ Ltac subtyping_tac :=
       try congruence
   end.
 
+
 #[tactic="subtyping_tac",derive(equations=no,eliminator=no)]
 Equations subtyping_nf_impl {P : PtsSig} (dec_P : DecidableSig P) (A : nf P) B : { {{ ⊢anf A ⊆ B }} } + {~ {{ ⊢anf A ⊆ B }} } :=
 | dec_P, n{{{ Sort@s }}}, n{{{ Sort@s' }}} =>
-    let*b _ := dec_st dec_P s s' while _ in
+    let*b _ := dec_st_sub dec_P s s' while _ in
     pureb _
 | dec_P, (@nf_pi P s1 s2 s3 r A B), (@nf_pi P s1' s2' s3' r' A' B') =>
     let*b _ := dec_st dec_P s1 s1' while _ in
     let*b _ := dec_st dec_P s2 s2' while _ in
     let*b _ := dec_st dec_P s3 s3' while _ in
-    let*b _ := dec_pi dec_P s1 s2 s3 r r' while _ in
+    let*b _ := strong_dec_pi dec_P s1 s1' s2 s2' s3 s3' r r' while _ in
     let*b _ := nf_eq_dec dec_P A A' while _ in
     let*b _ := subtyping_nf_impl dec_P B B' while _ in
     pureb _
@@ -41,28 +42,43 @@ Equations subtyping_nf_impl {P : PtsSig} (dec_P : DecidableSig P) (A : nf P) B :
   | left _ => left _
   | right _ => right _
   }.
-
+Next Obligation.
+assert (r = r').
+{
+  dependent destruction H0; reflexivity.
+}
+subst.
+unfold strong_ru_pi_eq in H.
+eapply H.
+repeat split; try reflexivity.
+Qed.
+Next Obligation.
+unfold strong_ru_pi_eq in s.
+destruct_conjs; subst.
+mauto 2.
+Qed.
+  
 (** The definitions of [subtyping_nf_impl] already come with soundness proofs,
     as well as obvious completeness. *)
 
-Theorem subtyping_nf_impl_complete : forall A B,
+Theorem subtyping_nf_impl_complete {P} (dec_P : DecidableSig P) : forall (A B : nf P),
     {{ ⊢anf A ⊆ B }} ->
-    exists H, subtyping_nf_impl A B = left H.
+    exists H, subtyping_nf_impl dec_P A B = left H.
 Proof.
   intros; dec_complete.
 Qed.
 
-Inductive subtyping_order G A B :=
+Inductive subtyping_order {P} (Γ : ctx P) A B :=
 | subtyping_order_run :
-  nbe_ty_order G A ->
-  nbe_ty_order G B ->
-  subtyping_order G A B.
+  nbe_ty_order Γ A ->
+  nbe_ty_order Γ B ->
+  subtyping_order Γ A B.
 #[local]
-Hint Constructors subtyping_order : mctt.
+Hint Constructors subtyping_order : mcpts.
 
-Lemma subtyping_order_sound : forall G A B,
-    {{ G ⊢a A ⊆ B }} ->
-    subtyping_order G A B.
+Lemma subtyping_order_sound {P} : forall (Γ : ctx P) A B,
+    {{ Γ ⊢a A ⊆ B }} ->
+    subtyping_order Γ A B.
 Proof.
   intros * H.
   dependent destruction H.
@@ -81,12 +97,12 @@ Ltac subtyping_impl_tac :=
   repeat subtyping_impl_tac1; try econstructor; mauto.
 
 #[tactic="subtyping_impl_tac",derive(equations=no,eliminator=no)]
-Equations subtyping_impl G A B (H : subtyping_order G A B) :
-  { {{G ⊢a A ⊆ B}} } + { ~ {{ G ⊢a A ⊆ B }} } :=
-| G, A, B, H =>
-    let (a, Ha) := nbe_ty_impl G A _ in
-    let (b, Hb) := nbe_ty_impl G B _ in
-    let*b _ := subtyping_nf_impl a b while _ in
+Equations subtyping_impl {P} (dec_P : DecidableSig P) (Γ : ctx P) A B (H : subtyping_order Γ A B) :
+  { {{ Γ ⊢a A ⊆ B }} } + { ~ {{ Γ ⊢a A ⊆ B }} } :=
+| dec_P, Γ, A, B, H =>
+    let (a, Ha) := nbe_ty_impl Γ A _ in
+    let (b, Hb) := nbe_ty_impl Γ B _ in
+    let*b _ := subtyping_nf_impl dec_P a b while _ in
     pureb _.
 Next Obligation.
   progressive_inversion.
@@ -96,20 +112,20 @@ Qed.
 
 (** Similar for [subtyping_impl]. *)
 
-Theorem subtyping_impl_complete' : forall G A B,
-    {{G ⊢a A ⊆ B}} ->
-    forall (H : subtyping_order G A B),
-      exists H', subtyping_impl G A B H = left H'.
+Theorem subtyping_impl_complete' {P} (dec_P : DecidableSig P) : forall (Γ : ctx P) A B,
+    {{Γ ⊢a A ⊆ B}} ->
+    forall (H : subtyping_order Γ A B),
+      exists H', subtyping_impl dec_P Γ A B H = left H'.
 Proof.
   intros; dec_complete.
 Qed.
 
 #[local]
-Hint Resolve subtyping_order_sound subtyping_impl_complete' : mctt.
+Hint Resolve subtyping_order_sound subtyping_impl_complete' : mcpts.
 
-Theorem subtyping_impl_complete : forall G A B,
-    {{G ⊢a A ⊆ B}} ->
-    exists H H', subtyping_impl G A B H = left H'.
+Theorem subtyping_impl_complete {P} (dec_P : DecidableSig P) : forall (Γ : ctx P) A B,
+    {{ Γ ⊢a A ⊆ B }} ->
+    exists H H', subtyping_impl dec_P Γ A B H = left H'.
 Proof.
   repeat unshelve mauto.
 Qed.
