theories/PtsSignature.v
@@ -132,208 +132,40 @@ End OrderProperties.
 Record DecidableSig (P : PtsSig) : Type :=
   mkDecidableSig {
       dec_st : forall (s s' : P), ( {s = s'} + {s <> s'} )%type;
-      dec_pi: forall (s1 s2 s3 : P) (r : Ru_pi P s1 s2 s3) (r' : Ru_pi P s1 s2 s3),
-        ( { r = r'} + {r <> r'} )%type
+      dec_ru_pi: forall (s1 s2 s3 : P) (r : Ru_pi P s1 s2 s3) (r' : Ru_pi P s1 s2 s3),
+        ( { r = r'} + {r <> r'} )%type;
+      dec_st_sub : forall (s s' : P), ({st_subtyp s s'} + {~ st_subtyp s s'})%type;
     }.
 Arguments dec_st {_}.
-Arguments dec_pi {_}.
+Arguments dec_ru_pi {_}.
+Arguments dec_st_sub {_}.
 
 Section DecidableProperties.
   Context {P : PtsSig} (dec_P : DecidableSig P).
 
-  Definition strong_equality (s1 s1' s2 s2' s3 s3' : P) (r : Ru_pi P s1 s2 s3) (r' : Ru_pi P s1' s2' s3') :=
+  Definition strong_ru_pi_eq (s1 s1' s2 s2' s3 s3' : P) (r : Ru_pi P s1 s2 s3) (r' : Ru_pi P s1' s2' s3') :=
       (s1 = s1') /\ (s2 = s2') /\ (s3 = s3') /\ (r ~= r').
 
-  Definition strong_inequality (s1 s1' s2 s2' s3 s3' : P) (r : Ru_pi P s1 s2 s3) (r' : Ru_pi P s1' s2' s3') :=
-    ~(strong_equality s1 s1' s2 s2' s3 s3' r r').
+  (* Definition strong_ru_pi_inequality (s1 s1' s2 s2' s3 s3' : P) (r : Ru_pi P s1 s2 s3) (r' : Ru_pi P s1' s2' s3') := *)
+  (*   ~(strong_ru_pi_eq s1 s1' s2 s2' s3 s3' r r'). *)
     
-  Lemma strong_decidable_pi : forall (s1 s1' s2 s2' s3 s3' : P) (r : Ru_pi P s1 s2 s3) (r' : Ru_pi P s1' s2' s3'),
-      ({ strong_equality s1 s1' s2 s2' s3 s3' r r' } + {strong_inequality s1 s1' s2 s2' s3 s3' r r'})%type.
+  Lemma strong_dec_pi : forall (s1 s1' s2 s2' s3 s3' : P) (r : Ru_pi P s1 s2 s3) (r' : Ru_pi P s1' s2' s3'),
+      ({ strong_ru_pi_eq s1 s1' s2 s2' s3 s3' r r' } + {~ strong_ru_pi_eq s1 s1' s2 s2' s3 s3' r r'})%type.
     intros.
-    destruct (dec_st dec_P s1 s1'); [| right; unfold strong_inequality; unfold strong_equality; intuition].
-    destruct (dec_st dec_P s2 s2'); [| right; unfold strong_inequality; unfold strong_equality; intuition].
-    destruct (dec_st dec_P s3 s3'); [| right; unfold strong_inequality; unfold strong_equality; intuition].
+    unfold strong_ru_pi_eq.
+    destruct (dec_st dec_P s1 s1'); [| right; intuition].
+    destruct (dec_st dec_P s2 s2'); [| right; intuition].
+    destruct (dec_st dec_P s3 s3'); [| right; intuition].
     subst.
-    destruct (dec_pi dec_P s1' s2' s3' r r').
+    destruct (dec_ru_pi dec_P s1' s2' s3' r r').
     - left.
-      unfold strong_equality.
-      repeat eexists.
+      repeat split.
       subst.
       reflexivity.
     - right.
-      unfold strong_inequality.
-      unfold strong_equality.
-      intros H.
-      destruct H as [? [? []]].
-      assert (r = r') by (eapply JMeq_eq; eassumption).
-      eauto.
-  Qed.
-End DecidableProperties.      
-
-
-(* Definition FullSig (P : PtsSig) : Type := forall s, exists s', Ax P s s'. *)
-
-
-(* Section SignatureExtension. *)
-(*   Context (P : PtsSig) (pred_P : PredicativeSig P). *)
-
-(*   (** Defining a new signature *) *)
-(*   Inductive eSt : Set := *)
-(*   | st_P : St P -> eSt *)
-(*   | st_ext : nat -> eSt. *)
-
-(*   Inductive eAx : eSt -> eSt -> Prop := *)
-(*   | ax_P : forall {s1 s2 : St P}, Ax P s1 s2 -> eAx (st_P s1) (st_P s2) *)
-(*   | ax_ext : forall {n : nat}, eAx (st_ext n) (st_ext (S n)) *)
-(*   | ax_cross : forall {s : St P}, eAx (st_P s) (st_ext 0). *)
-
-(*   Inductive eRu : eSt -> eSt -> eSt -> Set := *)
-(*   | ru_P : forall {s1 s2 s3 : St P}, Ru P s1 s2 s3 -> eRu (st_P s1) (st_P s2) (st_P s3). *)
-
-(*   Inductive eRu_nat : eSt -> Set := *)
-(*   | runat_P : forall {s : St P}, Ru_nat P s -> eRu_nat (st_P s). *)
-
-(*   Definition eP : PtsSig := mkPtsSig eSt eAx eRu eRu_nat. *)
-
-
-(*   (** Proof that the extended signature is still predicative *) *)
-(*   Inductive epred_rel : relation eP := *)
-(*   | pr_P : forall {s1 s2 : St P}, pred_rel pred_P s1 s2 -> epred_rel (st_P s1) (st_P s2) *)
-(*   | pr_ext : forall {i j : nat}, i < j -> epred_rel (st_ext i) (st_ext j) *)
-(*   | pr_cross : forall {s : St P} {i : nat}, epred_rel (st_P s) (st_ext i). *)
-
-
-(*   Lemma eord_rel : StrictOrder epred_rel. *)
-(*   Proof using Type. *)
-(*     assert (StrictOrder (pred_rel pred_P)) by (eapply ord_rel). *)
-(*     destruct H. *)
-(*     split. *)
-(*     - intros x Hx. *)
-(*       inversion_clear Hx. *)
-(*       + eapply StrictOrder_Irreflexive; eauto. *)
-(*       + unfold lt in H. *)
-(*         induction i. *)
-(*         * inversion H. *)
-(*         * eapply IHi. *)
-(*           eapply le_S_n; assumption. *)
-(*     - intros x y z Hxy. *)
-(*       inversion_clear Hxy; intros Hyz. *)
-(*       + inversion_clear Hyz. *)
-(*         * assert (pred_rel pred_P s1 s3) by (eapply StrictOrder_Transitive; eauto). *)
-(*           econstructor; auto. *)
-(*         * econstructor; auto. *)
-(*       + inversion_clear Hyz. *)
-(*         assert (i < j0) by (etransitivity; eauto). *)
-(*         econstructor; auto. *)
-(*       + inversion_clear Hyz. *)
-(*         econstructor; auto. *)
-(*   Qed. *)
-
-(*   Lemma wf_acc_orig : forall (s : P), Acc (pred_rel pred_P) s -> Acc epred_rel (st_P s). *)
-(*   Proof using Type. *)
-(*     intros. *)
-(*     induction H. *)
-(*     constructor. *)
-(*     intros. *)
-(*     assert (exists s' : P, y = (st_P s') /\ pred_rel pred_P s' x). *)
-(*     { *)
-(*       inversion H1; subst. *)
-(*       exists s1; split; auto. *)
-(*     } *)
-(*     destruct H2 as [s' []]. *)
-(*     rewrite H2. *)
-(*     apply H0. *)
-(*     assumption. *)
-(*   Qed. *)
-
-(*   Lemma wf_acc_nat : forall (i : nat), Acc lt i -> Acc epred_rel (st_ext i). *)
-(*   Proof using Type. *)
-(*     intros. *)
-(*     induction H. *)
-(*     constructor. *)
-(*     intros. *)
-(*     inversion H1; subst. *)
-(*     - apply H0; auto. *)
-(*     - apply wf_acc_orig. *)
-(*       apply (wf_rel pred_P). *)
-(*   Qed. *)
-
-(*   Lemma wf_acc_lt : forall (i : nat), Acc lt i. *)
-(*   Proof using Type. *)
-(*     intros i. *)
-(*     induction i; *)
-(*       constructor; intros. *)
-(*     - unfold lt in H. *)
-(*       inversion H. *)
-(*     - inversion H; auto. *)
-(*       destruct IHi; auto. *)
-(*   Qed. *)
-
-(*   Lemma epred_rel_wf : well_founded epred_rel. *)
-(*   Proof using Type. *)
-(*     assert (Hwf : well_founded (pred_rel pred_P)) by (apply wf_rel). *)
-(*     intros a. *)
-(*     constructor. *)
-(*     intros b H. *)
-(*     inversion_clear H. *)
-(*     - apply wf_acc_orig. *)
-(*       apply Hwf. *)
-(*     - apply wf_acc_nat. *)
-(*       apply wf_acc_lt. *)
-(*     - apply wf_acc_orig. *)
-(*       apply Hwf. *)
-(*   Qed. *)
-
-(*   Lemma eord_ax : forall (s1 s2 : eP), Ax eP s1 s2 -> epred_rel s1 s2. *)
-(*   Proof using Type. *)
-(*     intros. *)
-(*     inversion_clear H; econstructor; auto. *)
-(*     eapply ord_ax; assumption. *)
-(*   Qed. *)
-
-(*   Lemma eord_ru : forall (s1 s2 s3 : eP), Ru eP s1 s2 s3 -> (epred_rel s1 s3 \/ s1 = s3) /\ (epred_rel s2 s3 \/ s2 = s3). *)
-(*   Proof using Type. *)
-(*     intros. *)
-(*     inversion H; subst. *)
-(*     assert (((pred_rel pred_P s0 s5) \/ (s0 = s5)) /\ ((pred_rel pred_P s4 s5) \/ (s4 =s5))) by (apply ord_ru; auto). *)
-(*     destruct H1. *)
-(*     split. *)
-(*     - destruct H1. *)
-(*       + left. *)
-(*         econstructor; auto. *)
-(*       + right. *)
-(*         subst; reflexivity. *)
-(*     - destruct H2. *)
-(*       + left. *)
-(*         econstructor; auto. *)
-(*       + right. *)
-(*         subst; reflexivity. *)
-(*   Qed. *)
-
-
-(*   Definition epred_P : PredicativeSig eP := *)
-(*     mkPredicativeSig eP epred_rel eord_rel epred_rel_wf eord_ax eord_ru. *)
-
-(*   (** Proof that the extended signature is full *) *)
-(*   Lemma full_eP : FullSig eP. *)
-(*   Proof using Type. *)
-(*     intros s. *)
-(*     destruct s. *)
-(*     - exists (st_ext 0). *)
-(*       econstructor. *)
-
-(*     - exists (st_ext (S n)). *)
-(*       econstructor. *)
-(*   Qed. *)
-(* End SignatureExtension. *)
-
-(* Arguments st_P {P} s. *)
-(* Arguments st_ext {P} i. *)
-(* Arguments ax_P {P} {s1} {s2} ax. *)
-(* Arguments ax_ext {P} {n}. *)
-(* Arguments ax_cross {P} {s}. *)
-(* Arguments ru_P {P} {s1} {s2} {s3} ru. *)
-
-(* Arguments pr_P {P} {pred_P} {s1} {s2} pr. *)
-(* Arguments pr_ext {P} {pred_P} {i} {j} lt. *)
-(* Arguments pr_cross {P} {pred_P} {s} {i}. *)
+      intros [? [? []]].
+      subst.
+      eapply n.
+      reflexivity.
+  Qed.    
+End DecidableProperties.
