theories/Algorithmic/Typing.v
@@ -1,0 +1,1 @@
+From McPTS.Algorithmic.Typing Require Export Definitions Lemmas.
